fairneris/fuel_jm_scheduling_fairness.v
@@ -14,11 +14,11 @@ Section upto.
   Lemma upto_stutter_fairness_ltl (auxtr: auxtrace LM) (mtr: mtrace (joint_model M N)):
     upto_stutter_aux auxtr mtr ->
     (∀ ρ, fair_aux (LM := LM) ρ auxtr) →
-    fair_scheduling mtr.
+    jm_fair_scheduling mtr.
   Proof.
     intros Hupto Hfair ρ.
     opose proof (upto_stutter_fairness auxtr mtr _ _ (ρ: fmrole (joint_model M N))) as Hf=>//.
-    rewrite /fairness.fair_scheduling_mtr /fair_scheduling_mtr in Hf *.
+    rewrite /fairness.fair_scheduling_mtr /jm_fair_scheduling_mtr in Hf *.
     rewrite /trace_always_eventually_implies_now /trace_always_eventually_implies.
     rewrite trace_alwaysI. intros tr' [n Hsuff]. rewrite trace_impliesI. intros Hnow.
     rewrite /trace_utils.trace_implies in Hf. odestruct (Hf n _) as [m Hm].
